wip changing the representation of cfgs into gmaps

src/coq/Syntax/AstLib.v
@@ -7,289 +7,64 @@ From Vellvm Require Import
      Utilities
      Syntax.LLVMAst.
 
-From QuickChick Require Import Show.
+From stdpp Require Import gmap strings.
 
-Require Import Equalities OrderedType OrderedTypeEx.
-Require Import ExtLib.Core.RelDec ExtLib.Data.Z.
-Require Import ExtLib.Programming.Eqv.
-Require Import Ascii.
-
+Open Scope positive.
 Import ListNotations.
-Import EqvNotation.
 
 (* end hide *)
 
 (* Equalities --------------------------------------------------------------- *)
-#[global] Instance eq_dec_int : RelDec (@eq int) := Data.Z.RelDec_zeq.
-#[global] Instance eqv_int : Eqv int := (@eq int).
 
-(* These should be moved to part of the standard library, or at least to ExtLib *)
-Module AsciiOrd <: UsualOrderedType.
-  Definition t := ascii.
-  Definition eq := @eq t.
-  Definition eq_refl := @eq_refl t.
-  Definition eq_sym := @eq_sym t.
-  Definition eq_trans := @eq_trans t.
-  Definition lt (a b:ascii) := N.lt (N_of_ascii a) (N_of_ascii b).
-  Lemma lt_trans : forall a b c:t, lt a b -> lt b c -> lt a c.
-  Proof using.
-    intros a b c.
-    unfold lt.
-    apply N.lt_trans.
-  Qed.
-  Lemma lt_not_eq : forall a b:t, lt a b -> ~eq a b.
-  Proof using.
-    intros a b H.
-    unfold eq. unfold not. intros He. rewrite He in H.
-    eapply N.lt_neq. unfold lt in H. apply H. reflexivity.
-  Qed.
+#[global] Instance EqDecision_raw_id : EqDecision raw_id.
+solve_decision.
+Defined.
 
-  Lemma N_of_ascii_inj : forall x y, N_of_ascii x = N_of_ascii y -> x = y.
-  Proof using.
-    intros x y H.
-    rewrite <- ascii_N_embedding.
-    rewrite <- (@ascii_N_embedding x).
-    rewrite H. reflexivity.
-  Defined.
-
-  Program Definition compare (x y: t) : Compare lt eq x y :=
-    match N_as_OT.compare (N_of_ascii x) (N_of_ascii y) with
-    | LT p => _
-    | EQ p => _
-    | GT p => _
-    end.
-  Next Obligation.
-    apply LT. unfold lt. auto.
-  Defined.
-  Next Obligation.
-    apply EQ. unfold eq. apply N_of_ascii_inj. auto.
-  Defined.
-  Next Obligation.
-    apply GT. unfold lt. auto.
-  Defined.
-
-  Definition eq_dec := ascii_dec.
-End AsciiOrd.
-
-Module AsciiOrdFacts := OrderedTypeFacts(AsciiOrd).
-
-Module StringOrd <: UsualOrderedType.
-  Definition t := string.
-  Definition eq := @eq t.
-  Definition eq_refl := @eq_refl t.
-  Definition eq_sym := @eq_sym t.
-  Definition eq_trans := @eq_trans t.
-  Fixpoint lt (s1 s2:string) : Prop :=
-    match s1, s2 with
-    | EmptyString, EmptyString => False
-    | EmptyString, String _ _ => True
-    | String a s1', String b s2' =>
-      match AsciiOrd.compare a b with
-      | LT _ => True
-      | EQ _ => lt s1' s2'
-      | GT _ => False
+Definition Countable_raw_id_obligation :
+  ∀ x : raw_id,
+    match
+      match x with
+      | Name s => (encode s)~0~0
+      | Anon i => (encode i)~0~1
+      | Raw i => (encode i)~1~0
       end
-    | String _ _, EmptyString => False
-    end.
+    with
+    | p~0~1 => Anon <$> decode p
+    | p~1~0 => Raw <$> decode p
+    | p~0~0 => Name <$> decode p
+    | _ => None
+    end = Some x.
+Proof. now intros []; cbn; rewrite decode_encode. Qed.
 
-  Lemma lt_trans : forall a b c : t, lt a b -> lt b c -> lt a c.
-  Proof using.
-    induction a.
-    - destruct b; destruct c; simpl; intros; try tauto.
-    - destruct b; destruct c; simpl; intros; try tauto.
-      destruct (AsciiOrd.compare a a1); try tauto.
-      + destruct (AsciiOrd.compare a1 a2); try tauto.
-        * AsciiOrdFacts.elim_comp; auto.
-        * AsciiOrdFacts.elim_comp; auto.
-      + destruct (AsciiOrd.compare a1 a2); try tauto.
-        * AsciiOrdFacts.elim_comp; auto.
-        * AsciiOrdFacts.elim_comp; auto.
-          eapply IHa; eauto.
-  Qed.
+#[global] Instance Countable_raw_id : Countable raw_id :=
+  {|
+    encode id := match id with
+                 | Name s => (encode s)~0~0%positive
+                 | Anon i => (encode i)~0~1%positive
+                 | Raw  i => (encode i)~1~0%positive
+                 end;
+    decode p := match p with
+                | p~0~0 => Name <$> decode p
+                | p~0~1 => Anon <$> decode p
+                | p~1~0 => Raw  <$> decode p
+                | _     => None
+                end;
+    decode_encode := Countable_raw_id_obligation
+  |}.
 
-  Lemma lt_not_eq : forall a b:t, lt a b -> ~eq a b.
-  Proof using.
-    induction a; intros b H He; unfold eq in He; subst.
-    - unfold lt in H. destruct H.
-    - simpl in H.
-      destruct (AsciiOrd.compare a a); auto.
-      apply AsciiOrd.lt_not_eq in l. apply l. AsciiOrdFacts.order.
-      apply IHa in H. apply H. unfold eq. reflexivity.
-  Qed.
+#[global] Instance EqDecision_block_id : EqDecision block_id.
+solve_decision.
+Defined.
 
-  Program Fixpoint compare (s1 s2 : t) : Compare lt eq s1 s2 :=
-    match s1, s2 with
-    | EmptyString, EmptyString => _
-    | EmptyString, String b s2' => _
-    | String a s1', String b s2' =>
-      match AsciiOrd.compare a b with
-      | LT _ => _
-      | EQ _ => match compare s1' s2' with
-               | LT _ => _
-               | EQ _ => _
-               | GT _ => _
-               end
-      | GT _ => _
-      end
-    | String a s1', EmptyString => _
-    end.
-  Next Obligation.
-    apply EQ. unfold eq. reflexivity.
-  Defined.
-  Next Obligation.
-    apply LT. simpl. auto.
-  Defined.
-  Next Obligation.
-    apply LT. simpl. rewrite <- Heq_anonymous. auto.
-  Defined.
-  Next Obligation.
-    apply LT. simpl. rewrite <- Heq_anonymous0. auto.
-  Defined.
-  Next Obligation.
-    apply EQ. simpl. unfold AsciiOrd.eq in wildcard'0. subst. unfold eq in e. subst. reflexivity.
-  Defined.
-  Next Obligation.
-    apply GT. simpl. unfold AsciiOrd.eq in wildcard'0. subst.
-    rewrite <- Heq_anonymous0. auto.
-  Defined.
-  Next Obligation.
-    apply GT. simpl. AsciiOrdFacts.elim_comp_lt b a. auto.
-  Defined.
-  Next Obligation.
-    apply GT. simpl. auto.
-  Defined.
+#[global] Instance EqDecision_instr_id : EqDecision instr_id.
+solve_decision.
+Defined.
 
-  Definition eq_dec := string_dec.
-End StringOrd.
-Module StringOrdFacts := OrderedTypeFacts(StringOrd).
+#[global] Instance EqDecision_ident : EqDecision ident.
+solve_decision.
+Defined.
 
-
-Module RawIDOrd <: UsualOrderedType.
-  Definition t := raw_id.
-  Definition eq := @eq t.
-  Definition eq_refl := @eq_refl t.
-  Definition eq_sym := @eq_sym t.
-  Definition eq_trans := @eq_trans t.
-
-  (* Anon < Name < Raw *)
-  Definition lt (x:t) (y:t) : Prop :=
-    match x,y with
-    | Anon n1, Anon n2 => (n1 < n2)%Z
-    | Name s1, Name s2 => StringOrd.lt s1 s2
-    | Raw n1, Raw n2 => (n1 < n2)%Z
-    | Anon _, _ => True
-    | Name _, Raw _ => True
-    | _, _ => False
-    end.
-
-  Lemma lt_trans : forall a b c : t, lt a b -> lt b c -> lt a c.
-  Proof using.
-    destruct a; destruct b; destruct c; simpl; intros H1 H2; intuition.
-    - eapply StringOrd.lt_trans; eauto.
-  Qed.
-
-  Lemma lt_not_eq : forall a b:t, lt a b -> ~eq a b.
-  Proof using.
-    destruct a; destruct b; simpl; intros H He; inversion He; subst.
-    - apply StringOrd.lt_not_eq in H. apply H. unfold StringOrd.eq. reflexivity.
-    - apply Z_as_OT.lt_not_eq in H. tauto.
-    - apply Z_as_OT.lt_not_eq in H. tauto.
-  Qed.
-
-  Program Definition compare (x:t) (y:t) : Compare lt eq x y :=
-    match x,y with
-    | Anon n1, Anon n2 =>
-      match Z_as_OT.compare n1 n2 with
-      | LT _ => LT _
-      | EQ _ => EQ _
-      | GT _ => GT _
-      end
-    | Anon _, Name _ => LT _
-    | Anon _, Raw _ => LT _
-    | Name _, Anon _ => GT _
-    | Name s1, Name s2 =>
-      match StringOrd.compare s1 s2 with
-      | LT _ => LT _
-      | EQ _ => EQ _
-      | GT _ => GT _
-      end
-    | Name _, Raw _ => LT _
-    | Raw _, Anon _ => GT _
-    | Raw _, Name _ => GT _
-    | Raw n1, Raw n2 =>
-      match Z_as_OT.compare n1 n2 with
-      | LT _ => LT _
-      | EQ _ => EQ _
-      | GT _ => GT _
-      end
-    end.
-  Next Obligation.
-    unfold Z_as_OT.eq in wildcard'. subst. unfold eq. reflexivity.
-  Defined.
-  Next Obligation.
-    unfold StringOrd.eq in wildcard'. subst. unfold eq. reflexivity.
-  Defined.
-  Next Obligation.
-    unfold Z_as_OT.eq in wildcard'. subst. unfold eq. reflexivity.
-  Defined.
-
-  Definition eq_dec : forall (x y : t), {x = y} + {x <> y}.
-    decide equality.
-    - apply string_dec.
-    - apply rel_dec_p.
-    - apply rel_dec_p.
-  Defined.
-
-End RawIDOrd.
-
-#[global] Instance eq_dec_raw_id : RelDec (@eq raw_id) := RelDec_from_dec (@eq raw_id) RawIDOrd.eq_dec.
-#[global] Instance eqv_raw_id : Eqv raw_id := (@eq raw_id).
-#[export] Hint Unfold eqv_raw_id: core.
-
-Module InstrIDDec <: MiniDecidableType.
-  Definition t := instr_id.
-
-  Lemma eq_dec : forall (x y : instr_id), {x = y} + {x <> y}.
-  Proof using.
-    intros x y.
-    destruct x as [xn | xn]; destruct y as [yn | yn].
-    - destruct (xn ~=? yn). unfold eqv in e. unfold eqv_raw_id in e. subst. left. reflexivity.
-      right. unfold not. intros. apply n. inversion H. unfold eqv. unfold eqv_raw_id. reflexivity.
-    - right. unfold not. intros. inversion H.
-    - right. unfold not. intros. inversion H.
-    - destruct (xn ~=? yn).
-      left. unfold eqv in e. unfold eqv_int in e. subst. reflexivity.
-      right. unfold not. intros. apply n. inversion H. unfold eqv. unfold eqv_int. auto.
-  Defined.
-End InstrIDDec.
-Module InstrID := Make_UDT(InstrIDDec).
-
-#[global] Instance eq_dec_instr_id : RelDec (@eq instr_id) := RelDec_from_dec (@eq instr_id) InstrID.eq_dec.
-#[global] Instance eqv_instr_id : Eqv instr_id := (@eq instr_id).
-
-Module IdentDec <: MiniDecidableType.
-  Definition t := ident.
-
-  Lemma eq_dec : forall (x y : ident), {x = y} + {x <> y}.
-  Proof using.
-    intros x y.
-    destruct x as [xn | xn]; destruct y as [yn | yn].
-    - destruct (xn ~=? yn). unfold eqv in e. unfold eqv_raw_id in e. subst. left. reflexivity.
-      right. unfold not. intros. apply n. inversion H. unfold eqv. unfold eqv_raw_id. reflexivity.
-    - right. unfold not. intros. inversion H.
-    - right. unfold not. intros. inversion H.
-    - destruct (xn ~=? yn).
-      left. unfold eqv in e. unfold eqv_raw_id in e. subst.  reflexivity.
-      right. unfold not. intros. apply n. inversion H. unfold eqv. unfold eqv_raw_id. auto.
-  Defined.
-End IdentDec.
-Module Ident := Make_UDT(IdentDec).
-
-#[global] Instance eq_dec_ident : RelDec (@eq ident) := RelDec_from_dec (@eq ident) Ident.eq_dec.
-#[global] Instance eqv_ident : Eqv ident := (@eq ident).
-
-(* Induction Principles ----------------------------------------------------- *)
-
+(* Scheme Induction seems to still be too stupid to derive this automatically, fails to handle the nested lists  *)
 Section TypInd.
 
 Variable P : typ -> Prop.
@@ -499,246 +274,6 @@ Section ExpInd.
   Qed.
 End ExpInd.
 
-
-(* Display *)
-Require Import Ceres.Ceres.
-
-Section hiding_notation.
-  #[local] Open Scope sexp_scope.
-
-  Definition serialize_raw_id (prefix: string): Serialize raw_id :=
-    fun r =>
-      match r with
-      | Name s => Atom (prefix ++ s)%string
-      | Anon n => Atom (show_Z n)
-      | LLVMAst.Raw n => Atom ("_RAW_" ++ show_Z n)%string
-      end.
-
-  #[global] Instance serialize_raw_id': Serialize raw_id := serialize_raw_id "".
-
-  #[global] Instance serialize_ident : Serialize ident :=
-    fun id =>
-      match id with
-      | ID_Global r => serialize_raw_id "@" r
-      | ID_Local  r => serialize_raw_id "%" r
-      end.
-
-  #[global] Instance serialize_instr_id : Serialize instr_id :=
-    fun ins =>
-      match ins with
-      | IId id => serialize_raw_id "%" id
-      | IVoid n => Atom ("void<" ++ show_Z n ++ ">")%string
-      end.
-
-  #[global] Instance serialize_ibinop : Serialize ibinop :=
-    fun binop =>
-      match binop with
-      | LLVMAst.Add nuw nsw => Atom "add"
-      | Sub nuw nsw => Atom "sub"
-      | Mul nuw nsw => Atom "mul"
-      | Shl nuw nsw => Atom "shl"
-      | UDiv flag => Atom "udiv"
-      | SDiv flag => Atom "sdiv"
-      | LShr flag => Atom "lshr"
-      | AShr flag => Atom "ashr"
-      | URem | SRem => Atom "rem"
-      | And => Atom "and"
-      | Or => Atom "or"
-      | Xor => Atom "xor"
-      end.
-
-  #[global] Instance serialize_fbinop : Serialize fbinop :=
-    fun fbinop =>
-      match fbinop with
-      | FAdd => Atom "fadd"
-      | FSub => Atom "fsub"
-      | FMul => Atom "fmul"
-      | FDiv => Atom "fdiv"
-      | FRem => Atom "frem"
-      end.
-
-  #[global] Instance serialize_icmp : Serialize icmp :=
-    fun cmp =>
-      Atom ("icmp "
-             ++
-             match cmp with
-             | Eq => "eq"
-             | Ne => "ne"
-             | Ugt => "ugt"
-             | Uge => "uge"
-             | Ult => "ult"
-             | Ule => "ule"
-             | Sgt => "sgt"
-             | Sge => "sge"
-             | Slt => "slt"
-             | Sle => "sle"
-             end)%string.
-
-  #[global] Instance serialize_fcmp : Serialize fcmp :=
-    fun cmp =>
-      Atom ("fcmp "
-             ++
-             match cmp with
-               FFalse => "ffalse"
-             | FOeq => "foeq"
-             | FOgt => "fogt"
-             | FOge => "foge"
-             | FOlt => "folt"
-             | FOle => "fole"
-             | FOne => "fone"
-             | FOrd => "ford"
-             | FUno => "funo"
-             | FUeq => "fueq"
-             | FUgt => "fugt"
-             | FUge => "fuge"
-             | FUlt => "fult"
-             | FUle => "fule"
-             | FUne => "fune"
-             | FTrue => "ftrue"
-             end)%string.
-
-  (* I need show_ZVellvm here because Ceres segfaults on extraction for
-  showing integers for some reason *)
-  Fixpoint serialize_typ' typ: sexp :=
-    match typ with
-    | TYPE_I sz => Atom ("i" ++ show_N sz)%string
-    | TYPE_IPTR => Atom ("iptr")%string
-    | TYPE_Pointer t => [serialize_typ' t ; Atom "*"]
-    | TYPE_Void => Atom "void"
-    | TYPE_Half => Atom "half"
-    | TYPE_Float => Atom "float"
-    | TYPE_Double => Atom "double"
-    | TYPE_X86_fp80 => Atom "x86_fp80"
-    | TYPE_Fp128 => Atom "fp128"
-    | TYPE_Ppc_fp128 => Atom "ppc_fp128"
-    | TYPE_Metadata => Atom "metadata"
-    | TYPE_X86_mmx => Atom "x86_mmx"
-    | TYPE_Array sz t => [Atom "["; Atom (show_N sz); Atom "x"; serialize_typ' t; Atom "]"]
-    | TYPE_Function ret args varargs => [serialize_typ' ret; Atom "("; Atom (String.concat ", " (map (fun x => CeresFormat.string_of_sexp (serialize_typ' x)) args)); Atom ")"]
-    | TYPE_Struct fields => [Atom "{"; Atom (String.concat ", " (map (fun x => CeresFormat.string_of_sexp (serialize_typ' x)) fields)); Atom "}"]
-    | TYPE_Packed_struct fields => [Atom "<{"; Atom (String.concat ", " (map (fun x => CeresFormat.string_of_sexp (serialize_typ' x)) fields)); Atom "}>"]
-    | TYPE_Opaque => Atom "opaque"
-    | TYPE_Vector sz t => [Atom "<"; Atom (show_N sz); Atom "x"; serialize_typ' t; Atom ">"]
-    | TYPE_Identified id => Atom (to_string id)
-    end.
-
-  #[global] Instance serialize_typ : Serialize typ := serialize_typ'.
-
-  Section WithSerializeT.
-    Variable (T:Set).
-    Context `{serializeT : Serialize T}.
-
-    Fixpoint serialize_exp' (v : exp T) :=
-      match v with
-      | EXP_Ident id => to_sexp id
-      | EXP_Integer x => Atom (show_Z x)
-      | EXP_Bool b => to_sexp b
-      | EXP_Null => Atom "null"
-      | EXP_Zero_initializer => Atom "zero initializer"
-      | EXP_Undef => Atom "undef"
-      | OP_IBinop iop t v1 v2 =>
-        [to_sexp iop ; to_sexp t
-                    ; serialize_exp' v1
-                    ; serialize_exp' v2]
-      | OP_ICmp cmp t v1 v2 =>
-        [to_sexp cmp ; to_sexp t
-                    ; serialize_exp' v1
-                    ; serialize_exp' v2]
-      | OP_GetElementPtr t ptrval idxs =>
-        Atom "getelementptr"
-      | _ => Atom "to_sexp_exp todo"
-      end.
-
-    #[global] Instance serialize_exp : Serialize (exp T) := serialize_exp'.
-    #[global] Instance serialize_int : Serialize int := fun i => Atom (show_Z i).
-
-    #[global] Instance serialize_texp : Serialize (texp T) :=
-      fun '(t, e) =>
-          [to_sexp t ; Atom " " ; to_sexp e ].
-
-    Definition serialize_opt {A:Type} `{AS:Serialize A} (s:string) : Serialize (option A) :=
-      fun x =>
-        match x with
-        | None => Atom ""
-        | Some a => [Atom s ; to_sexp a]
-        end.
-
-    #[global] Instance serialize_instr : Serialize (instr T) :=
-      fun instr =>
-        match instr with
-          (* SAZ: OUT OF DATE *)
-        (*
-        | INSTR_Op op => to_sexp op
-
-        | INSTR_Load t ptr anns =>
-          [Atom "load" ; to_sexp t ; to_sexp ptr ]
-
-        | INSTR_Store tval ptr anns =>
-          [Atom "store" ; to_sexp tval; to_sexp ptr
-           ; @serialize_opt _ serialize_int ", align" align]
-
-        | INSTR_Alloca t anns (* TODO: add anns *)=>
-          [Atom "alloca" ; to_sexp t]
-
-           | INSTR_Call
-           | INSTR_Phi
-           | INSTR_Alloca
-         *)
-        | _ => Atom "string_of_instr todo"
-        end.
-
-    #[global] Instance serialize_terminator : Serialize (terminator T) :=
-      fun t =>
-        match t with
-        | TERM_Ret v => [Atom "ret " ; to_sexp v]
-        | TERM_Ret_void => Atom "ret"
-        | TERM_Br te b1 b2 =>
-          [Atom "br"; to_sexp te; Atom ", label "; to_sexp b1; Atom ", label "; to_sexp b2]
-        | TERM_Br_1 b => [Atom "br label"; to_sexp b]
-        | _ => Atom "string_of_terminator todo"
-        end.
-
-    #[global] Instance serialize_instr_id_instr : Serialize (instr_id * (instr T)) :=
-      fun '(iid, i) =>
-        match iid with
-        | IId _ =>
-          [to_sexp iid ; Atom "=" ; to_sexp i]
-        | IVoid n =>
-          [to_sexp i]
-        end.
-
-    #[global] Instance serialize_block : Serialize (block T) :=
-      fun block =>
-        [to_sexp (blk_id block) ; Atom ":\n" ;
-        (* TODO: add indentation *)
-        to_sexp (blk_code block); to_sexp (blk_term block)].
-  End WithSerializeT.
-
-  (* TODO: What is this SerializeTyp stuff about? Why use ceres? *)
-  Section SerializeTyp.
-    #[global] Instance serialize_definition_list_block : Serialize (definition typ (list (block typ))) :=
-      fun defn =>
-        match defn.(df_prototype).(dc_type) with
-        | TYPE_Function ret_t args_t varargs
-          => let name  := defn.(df_prototype).(dc_name) in
-             [Atom "define"; to_sexp ret_t; to_sexp name;
-             Atom " {\n";
-             (* TODO: Add prefix for indentation? *)
-             to_sexp (df_instrs defn);
-             Atom "}\n"]
-        | _ => Atom "Invalid type on function"
-        end.
-
-    #[global] Instance serialize_tle_list_block : Serialize (toplevel_entity typ (list (block typ))) :=
-      fun tle =>
-        match tle with
-        | TLE_Definition defn => to_sexp defn
-        | _ => Atom "string_of_tle_list_block todo"
-        end.
-  End SerializeTyp.
-End hiding_notation.
-
-
 (* Utility function to determine whether a typ is void or is a function type returning void.
    This is needed in the parser to determine whether a function call instruction should
    generate an "anonymous" id or a "void" id.
@@ -762,9 +297,6 @@ Definition is_void_instr (i:instr typ) : bool :=
   | INSTR_Store _ _ _ => true
   | _ => false
   end.
-
-Ltac unfold_eqv :=
-  repeat (unfold eqv in *; unfold eqv_raw_id in *; unfold eqv_instr_id in * ).
 
 (* This function extracts the string of the form [llvm._] from an LLVM expression.
    It returns None if the expression is not an intrinsic definition.
