src/coq/Syntax/Scope.v
@@ -2,14 +2,14 @@
 From Coq Require Import
      List.
 Import ListNotations.
-
+From stdpp Require Import fin_maps fin_map_dom gmap mapset.
 From Vellvm Require Import
      Numeric.Coqlib
      Utilities
      Syntax.LLVMAst
+     Syntax.AstLib
      Syntax.CFG
      Syntax.TypToDtyp.
-
 
 (* end hide *)
 
@@ -37,51 +37,48 @@ Section LABELS_OPERATIONS.
      Denoting an [ocfg] starting from a label out of this static list
      always results in the identity.
    *)
-  Definition inputs (ocfg : @ocfg T) :=
-    map blk_id ocfg.
+  Definition inputs (ocfg : @ocfg T) := dom ocfg.
 
   (** * outputs
      Collect the list of output labels in an open control flow graph.
      Denoting an [ocfg] starting from a label that belongs to its [inputs]
      will always result in a label in the static [output] list, or in a value.
    *)
-  Definition terminator_outputs (term : terminator T) : list block_id
+  Definition terminator_outputs (term : terminator T) : gset block_id
     := match term with
-       | TERM_Ret v => []
-       | TERM_Ret_void => []
-       | TERM_Br v br1 br2 => [br1; br2]
-       | TERM_Br_1 br => [br]
-       | TERM_Switch v default_dest brs => default_dest :: map snd brs
-       | TERM_IndirectBr v brs => brs
-       | TERM_Resume v => []
-       | TERM_Invoke fnptrval args to_label unwind_label => [to_label; unwind_label]
-       | TERM_Unreachable => []
+       | TERM_Ret v => ∅
+       | TERM_Ret_void => ∅
+       | TERM_Br v br1 br2 => {[br1; br2]}
+       | TERM_Br_1 br => {[br]}
+       | TERM_Switch v default_dest brs => {[default_dest]} ∪ list_to_set (map snd brs)
+       | TERM_IndirectBr v brs => list_to_set brs
+       | TERM_Resume v => ∅
+       | TERM_Invoke fnptrval args to_label unwind_label => {[to_label; unwind_label]}
+       | TERM_Unreachable => ∅
        end.
 
-  Definition successors (bk : block T) : list block_id :=
+  Definition successors (bk : block T) : gset block_id :=
     terminator_outputs (blk_term bk).
 
-  Definition outputs (bks : ocfg T) : list block_id
-    := fold_left (fun acc bk => acc ++ successors bk) bks [].
+  Definition outputs (bks : ocfg T) : gset block_id
+    := map_fold (fun _ bk acc => acc ∪ successors bk) ∅ bks.
 
-  Lemma raw_id_eq_dec : forall (x y : raw_id), {x = y} + {x <> y}.
-  Proof using.
-    intros. destruct (Eqv.eqv_dec_p x y); auto.
-  Qed.
-
-  Definition raw_id_in := in_dec raw_id_eq_dec.
+  (* Definition raw_id_in := elem_of_list_dec (A := raw_id). *)
 
   (* Test whether b ∈ successors(bk), i.e.
   [is_predecessor b bk] iff [bk] is a predecessor to [b].
    *)
   Definition is_predecessor (b : block_id) (bk : block T) : bool :=
-    if raw_id_in b (successors bk) then true else false.
+    if decide (elem_of b (successors bk)) then true else false.
 
-  (* Computes the set of predecessors of [b] in [G] *)
+  (* Computes the set of predecessors of [b] in [G].
+   *)
 
-  Definition predecessors (b : block_id) (G : ocfg T) : list block_id :=
-    fold_left (fun acc bk => if is_predecessor b bk then bk.(blk_id) :: acc else acc) G [].
+  Definition predecessors (b : block_id) (bks : ocfg T) : list block_id :=
+    map_fold (fun k bk acc => if is_predecessor b bk then k :: acc else acc) [] bks.
 
+  (* Now by construction since we represent graphs as finmaps *)
+  (*
   (** * well-formed
       All labels in an open cfg are distinct.
       Quite natural sanity condition ensuring that despite the representation of
@@ -90,6 +87,7 @@ Section LABELS_OPERATIONS.
    *)
   Definition wf_ocfg_bid (bks : ocfg T) : Prop :=
     list_norepet (inputs bks).
+   *)
 
   (** * no reentrance
       Generally speaking, all blocks in an open cfg are mutually recursive,
@@ -105,14 +103,14 @@ Section LABELS_OPERATIONS.
       notably.
    *)
   Definition no_reentrance (bks1 bks2 : ocfg T) : Prop :=
-    outputs bks2 ⊍ inputs bks1.
+    outputs bks2 ## inputs bks1.
 
   (** * no_duplicate_bid
       Checks that the inputs of two sub-graphs are disjoint. This condition ensures
       that the well formedness of the two computations entails the one of their join.
    *)
   Definition no_duplicate_bid (bks1 bks2 : ocfg T) : Prop :=
-    inputs bks1 ⊍ inputs bks2.
+    inputs bks1 ## inputs bks2.
 
   (** * independent
       While [no_reentrance] captures two sequential computations,
@@ -126,26 +124,26 @@ Section LABELS_OPERATIONS.
     no_duplicate_bid bks1 bks2.
 
   Definition free_in_cfg (cfg : ocfg T ) (id : block_id) : Prop :=
-    not (In id (inputs cfg)).
+    ~ (elem_of id (inputs cfg)).
 
-  Definition phi_sources (φ : phi T) : list block_id :=
-    let '(Phi _ l) := φ in map fst l.
+  Definition phi_sources (φ : phi T) : gset block_id :=
+    let '(Phi _ l) := φ in list_to_set (map fst l).
 
   (* Over a closed graph, phi nodes should expect exactly jumps from their predecessors:
      - For any block [bk] in the graph
      - For any phi node [phi] in this block
      - the sources of [phi] and the predecessors of [bk] are in bijection
    *)
-  Definition wf_ocfg_phis (G : ocfg T) :=
-    forall bk pred x phi,
-      In bk G ->
-      In (x,phi) bk.(blk_phis) ->
-      (In pred (phi_sources phi) <-> In pred (predecessors bk.(blk_id) G)).
+  Definition wf_ocfg_phis (bks : ocfg T) : Prop :=
+    map_Forall
+      (fun id bk => forall x φ pred, elem_of (x,φ) bk.(blk_phis) ->
+                             (elem_of pred (phi_sources φ) <-> elem_of pred (predecessors id bks)))
+      bks.
 
   Record wf_cfg (G : cfg T): Prop :=
     WF_CFG
       {
-        wf_cfg_bid : wf_ocfg_bid G.(blks);
+        (* wf_cfg_bid : wf_ocfg_bid G.(blks); *)
         wf_cfg_phis : wf_ocfg_phis G.(blks)
       }.
 
@@ -155,52 +153,57 @@ End LABELS_OPERATIONS.
     Once things are a bit settled, we need to use a more efficient implementation of
     sets ([MSetRBT.v] for instance)
  *)
-From Coq Require Import ListSet.
 
-Module SetNotations.
 
-  Infix "+++" := (set_union raw_id_eq_dec) (right associativity, at level 60).
-  Infix ":::" := (set_add raw_id_eq_dec) (right associativity, at level 60).
-  Infix "∖"    := (set_diff raw_id_eq_dec) (right associativity, at level 60).
-  Notation "∅" := (empty_set _).
+(* From Coq Require Import ListSet. *)
 
-  Definition set_flat_map {A} (f : A -> set raw_id) :=
-    fix flat_map (l:set A) : set raw_id :=
-      match l with
-      | nil => nil
-      | cons x t => (f x) +++ (flat_map t)
-      end.
+(* Module SetNotations. *)
 
-End SetNotations.
+(*   Infix "+++" := (set_union raw_id_eq_dec) (right associativity, at level 60). *)
+(*   Infix ":::" := (set_add raw_id_eq_dec) (right associativity, at level 60). *)
+(*   Infix "∖"    := (set_diff raw_id_eq_dec) (right associativity, at level 60). *)
+(*   Notation "∅" := (empty_set _). *)
 
-Import SetNotations.
+(*   Definition set_flat_map {A} (f : A -> set raw_id) := *)
+(*     fix flat_map (l:set A) : set raw_id := *)
+(*       match l with *)
+(*       | nil => nil *)
+(*       | cons x t => (f x) +++ (flat_map t) *)
+(*       end. *)
+
+(* End SetNotations. *)
+
+(* Import SetNotations. *)
 
 Section REGISTER_OPERATIONS.
+
+  Definition set_flat_map_list {A B} `{EqDecision B, Countable B} (f : A -> gset B) (l : list A) : gset B :=
+    foldl (fun acc x => f x ∪ acc) ∅ l.
 
   Section Defs.
 
     (** * Definition sites
       Simple static collection of all variables assigned to in a piece of syntax.
      *)
-    Class Def_sites (A : Type) := { def_sites: A -> set raw_id }.
-
+    Class Def_sites (A : Type) := { def_sites: A -> gset raw_id }.
 
     #[global] Instance instr_id_defs : Def_sites instr_id :=
       {| def_sites := fun id =>
                         match id with
-                        | IId id => [id]
+                        | IId id => {[id]}
                         | _ => ∅
                         end |}
     .
 
     #[global] Instance code_defs {T} : Def_sites (code T) :=
-      {| def_sites := fold_right (fun '(id,_) acc => def_sites id +++ acc) ∅ |}.
+      {| def_sites := set_flat_map_list (fun x => def_sites (fst x)) |}.
 
     #[global] Instance block_def_sites {T} : Def_sites (block T) :=
-      {| def_sites := fun bk => map fst bk.(blk_phis) +++ def_sites bk.(blk_code) |}.
+      {| def_sites := fun bk => list_to_set (map fst bk.(blk_phis)) ∪
+                             def_sites bk.(blk_code) |}.
 
     #[global] Instance ocfg_def_sites {T} : Def_sites (ocfg T) :=
-      {| def_sites := set_flat_map def_sites |}.
+      {| def_sites := map_fold (fun k bk acc => def_sites bk ∪ acc) ∅ |}.
 
     #[global] Instance cfg_def_sites {T} : Def_sites (cfg T) :=
       {| def_sites := fun cfg => def_sites cfg.(blks) |}.
@@ -213,55 +216,55 @@ Section REGISTER_OPERATIONS.
         Simple static collection of all local variables read in a piece of syntax.
      *)
 
-    Class Use_sites (A : Type) := { use_sites: A -> set raw_id }.
+    Class Use_sites (A : Type) := { use_sites: A -> gset raw_id }.
 
     #[global] Instance ident_use_sites : Use_sites ident :=
-      {| use_sites := fun id => match id with | ID_Local id => [id] | ID_Global _ => ∅ end |}.
+      {| use_sites := fun id => match id with | ID_Local id => {[id]} | ID_Global _ => ∅ end |}.
 
     #[global] Instance exp_use_sites {T} : Use_sites (exp T) :=
       {| use_sites :=
-           fix f e := match e with
-                      | EXP_Ident id
-                        => use_sites id
+          fix f e := match e with
+                     | EXP_Ident id
+                       => use_sites id
 
-                      | EXP_Integer _
-                      | EXP_Float _
-                      | EXP_Double _
-                      | EXP_Hex _
-                      | EXP_Bool _
-                      | EXP_Null
-                      | EXP_Zero_initializer
-                      | EXP_Cstring _
-                      | EXP_Undef
-                        => []
+                     | EXP_Integer _
+                     | EXP_Float _
+                     | EXP_Double _
+                     | EXP_Hex _
+                     | EXP_Bool _
+                     | EXP_Null
+                     | EXP_Zero_initializer
+                     | EXP_Cstring _
+                     | EXP_Undef
+                       => ∅
 
-                      | OP_Conversion _ _ e _
-                      | OP_ExtractValue (_,e) _
-                      | OP_Freeze (_,e)
-                        => f e
+                     | OP_Conversion _ _ e _
+                     | OP_ExtractValue (_,e) _
+                     | OP_Freeze (_,e)
+                       => f e
 
-                      | OP_IBinop _ _ e1 e2
-                      | OP_ICmp _ _ e1 e2
-                      | OP_FBinop _ _ _ e1 e2
-                      | OP_FCmp _ _ e1 e2
-                      | OP_ExtractElement (_,e1) (_,e2)
-                      | OP_InsertValue (_,e1) (_,e2) _
-                        => f e1 +++ f e2
+                     | OP_IBinop _ _ e1 e2
+                     | OP_ICmp _ _ e1 e2
+                     | OP_FBinop _ _ _ e1 e2
+                     | OP_FCmp _ _ e1 e2
+                     | OP_ExtractElement (_,e1) (_,e2)
+                     | OP_InsertValue (_,e1) (_,e2) _
+                       => f e1 ∪ f e2
 
-                      | OP_InsertElement (_,e1) (_,e2) (_,e3)
-                      | OP_ShuffleVector (_,e1) (_,e2) (_,e3)
-                      | OP_Select (_,e1) (_,e2) (_,e3)
-                        => f e1 +++ f e2 +++ f e3
+                     | OP_InsertElement (_,e1) (_,e2) (_,e3)
+                     | OP_ShuffleVector (_,e1) (_,e2) (_,e3)
+                     | OP_Select (_,e1) (_,e2) (_,e3)
+                       => f e1 ∪ f e2 ∪ f e3
 
-                      | EXP_Struct l
-                      | EXP_Packed_struct l
-                      | EXP_Array l
-                      | EXP_Vector l
-                        => set_flat_map (fun x => f (snd x)) l
+                     | EXP_Struct l
+                     | EXP_Packed_struct l
+                     | EXP_Array l
+                     | EXP_Vector l
+                       => set_flat_map_list (fun x => f (snd x)) l
 
-                      | OP_GetElementPtr _ (_,e) l
-                        => f e +++ set_flat_map (fun x => f (snd x)) l
-                      end
+                     | OP_GetElementPtr _ (_,e) l
+                       => f e ∪ set_flat_map_list (fun x => f (snd x)) l
+                     end
       |}.
 
     #[global] Instance texp_use_sites {T} : Use_sites (texp T) := {| use_sites := fun x => use_sites (snd x) |}.
@@ -270,12 +273,13 @@ Section REGISTER_OPERATIONS.
     #[global] Instance instr_use_sites {T} : Use_sites (instr T) :=
       {| use_sites := fun i => match i with
                             | INSTR_Op e => use_sites e
-                            | INSTR_Call e l _ => use_sites (e:texp T) +++
-                                                   set_flat_map use_sites (List.map fst l)
+                            | INSTR_Call e l _ =>
+                                use_sites (e:texp T) ∪
+                                  set_flat_map_list (fun x => use_sites (fst x)) l
                             | INSTR_Load  _ e _
                               => use_sites e
                             | INSTR_Store e1 e2 _
-                              => use_sites e1 +++ use_sites e2
+                              => use_sites e1 ∪ use_sites e2
                             | INSTR_Alloca _ _
                             | INSTR_Fence _ _
                             | INSTR_AtomicCmpXchg _
@@ -283,12 +287,12 @@ Section REGISTER_OPERATIONS.
                             | INSTR_VAArg _ _
                             | INSTR_LandingPad
                             | INSTR_Comment _
-                              => []
+                              => ∅
                             end
       |}.
 
     #[global] Instance code_use_sites {T} : Use_sites (code T) :=
-      {| use_sites := set_flat_map (fun x => use_sites (snd x)) |}.
+      {| use_sites := set_flat_map_list (fun x => use_sites (snd x)) |}.
 
     #[global] Instance term_use_sites {T} : Use_sites (terminator T) :=
       {| use_sites := fun t => match t with
@@ -304,24 +308,27 @@ Section REGISTER_OPERATIONS.
                                | TERM_Ret_void
                                | TERM_Br_1 _
                                | TERM_Unreachable
-                                 => []
+                                 => ∅
 
                                | TERM_Invoke _ l _ _ =>
-                                 set_flat_map use_sites (List.map fst l)
+                                 set_flat_map_list (fun x => use_sites (fst x)) l
                                end
       |}.
 
     #[global] Instance phi_use_sites {T} : Use_sites (phi T) :=
-      {| use_sites := fun '(Phi _ l) => set_flat_map (fun x => use_sites (snd x)) l |}.
+      {| use_sites := fun '(Phi _ l) => set_flat_map_list (fun x => use_sites (snd x)) l |}.
 
     #[global] Instance block_use_sites {T} : Use_sites (block T) :=
-      {| use_sites := fun bk => set_flat_map (fun x => use_sites (snd x)) bk.(blk_phis) +++ use_sites bk.(blk_code) +++ use_sites bk.(blk_term) |}.
+      {| use_sites bk :=
+          set_flat_map_list (fun x => use_sites (snd x)) bk.(blk_phis)
+        ∪ use_sites bk.(blk_code)
+        ∪ use_sites bk.(blk_term) |}.
 
     #[global] Instance ocfg_use_sites {T} : Use_sites (ocfg T) :=
-      {| use_sites := set_flat_map use_sites |}.
+      {| use_sites := map_fold (fun k bk acc => use_sites bk ∪ acc) ∅ |}.
 
     #[global] Instance cfg_use_sites {T} : Use_sites (cfg T) :=
-      {| use_sites := fun cfg => cfg.(args) +++ use_sites cfg.(blks) |}.
+      {| use_sites := fun cfg => list_to_set cfg.(args) ∪ use_sites cfg.(blks) |}.
 
   End Uses.
 
